\documentclass[a4paper]{article}

\usepackage[paperwidth=21cm, paperheight=31cm, margin=0.2cm]{geometry}
\usepackage{amsmath}
\usepackage{amssymb}
\usepackage{amsfonts}
\usepackage{xcolor}
\usepackage{titlesec}
\titleformat*{\section}{\Huge\bfseries}
\titlespacing*{\section}
{0pt}{5.5ex plus 1ex minus .2ex}{4.3ex plus .2ex}
\titlespacing*{\subsection}
{0pt}{5.5ex plus 1ex minus .2ex}{4.3ex plus .2ex}


\begin{document}
\Large
\section*{(a)  $\cos(\alpha - \beta) = \cos\alpha\cos\beta + \sin\alpha\sin\beta$}

From the law of cosines,

\begin{equation}
  |\vec{a} - \vec{b}|^2 = |\vec{a}|^2 + |\vec{b}|^2 - 2|\vec{a}||\vec{b}|\cos(\alpha - \beta) 
\end{equation}
\\

$\begin{array}{rcl}
	| \vec{a} - \vec{b} |^2  & = & (a \cos \alpha - b \cos \beta)^2 - (a \sin \alpha - b \sin \beta)^2 \\
\\
	& = & ( a^2\cos^2\alpha - 2ab \cos\alpha\cos\beta + b^2\cos^2\beta) + (a^2\sin\alpha - 2ab\sin\alpha\sin\beta + b^2\sin^2\beta) \\
\\
	& = & a^2 + b^2 - 2ab(\cos\alpha\cos\beta+\sin\alpha\sin\beta
\end{array}
$\\\\

$
|\vec{a}|^2+|\vec{b}|^2-2|\vec{a}||\vec{b}|\cos(\alpha-\beta) = a^2 + b^2 - 2ab\cos(\alpha-\beta) 
$
\\\\

$
\therefore \ \cos (\alpha - \beta) = \cos\alpha \cos \beta - \sin \alpha \sin \beta
$

\section*{(b)  $ \sin (\alpha - \beta) = \sin\alpha \cos \beta - \cos \alpha \sin \beta $}

From the Pythagorean identity, 

\begin{equation}
  \sin^2(\alpha-\beta)+\cos^2(\alpha-\beta) = 1
\end{equation}
\\

$
\begin{array}{rcl}
\sin(\alpha-\beta) & = & \sqrt{1-\cos^2(\alpha-\beta)} \\\\
& = & \sqrt{1-(\cos\alpha\cos\beta+\sin\alpha\sin\beta)^2} \\\\
& = & \sqrt{1-(\cos^2\alpha\cos^2\beta+2\cos\alpha\cos\beta\sin\alpha\sin\beta+\sin^2\alpha\sin^2\beta)} \\\\
& = & \sqrt{1-\{\cos^2\alpha(1-\sin^2\beta)+2\cos\alpha\cos\beta\sin\alpha\sin\beta+\sin^2\alpha(1-\cos^2\beta)\}} \\\\
& = & \sqrt{1-(\cos^2\alpha-\cos^2\alpha\sin^2\beta+2\cos\alpha\cos\beta\sin\alpha\sin\beta+\sin^2\alpha-\sin^2\alpha\cos^2\beta)} \\\\
& = & \sqrt{\cos^2\alpha\sin^2\beta-2\cos\alpha\cos\beta\sin\alpha\sin\beta+\sin^2\alpha\cos^2\beta} \\\\
& = & \sqrt{(\cos\alpha\sin\beta-\sin\alpha\cos\beta)^2} \\\\
& = & \cos\alpha\sin\beta-\sin\alpha\cos\beta
\end{array}	
$
\\\\

$
\therefore \ \sin(\alpha-\beta) = \cos\alpha\sin\beta-\sin\alpha\cos\beta
$

\end{document}